theories/Sorted.v
@@ -8,39 +8,50 @@ Open Scope Z_scope.
 
 Module Sorted.
 
-Inductive sorted : list int -> Prop :=
+Inductive sorted {V: Type} : list (int*V) -> Prop :=
     | sorted_nil :
         sorted []
-    | sorted_1 : forall x,
-        sorted [x]
-    | sorted_cons : forall x y l,
-        mk_z x <= mk_z y -> sorted (y :: l) -> sorted (x :: y :: l).
+    | sorted_1 : forall x v,
+        sorted [(x,v)]
+    | sorted_cons : forall x vx y vy l,
+        mk_z x <= mk_z y -> sorted ((y, vy) :: l) -> sorted ((x, vx) :: (y, vy) :: l).
 
 
-Lemma sorted_app: forall l1 l2 x,
+Lemma sorted_app {V: Type} : forall l1 l2 x (vx: V),
     sorted l1 -> sorted l2 ->
-    Forall (fun n => mk_z n < mk_z x) l1 -> Forall (fun n => mk_z n > mk_z x) l2 ->
-    sorted (l1 ++ x :: l2).
+    Forall (fun '(n, _) => mk_z n < mk_z x) l1 -> Forall (fun '(n,_) => mk_z n > mk_z x) l2 ->
+    sorted (l1 ++ (x, vx) :: l2).
 Proof.
     intros l1 l2 x Hl1 Hl2 Hlt Hgt.
     induction l1 as [|h t IHt].
-    - rewrite app_nil_l.
+    - intros. rewrite app_nil_l.
       inversion Hl2; clear Hl2; subst. 
       repeat constructor.
-      + constructor.
-      ++ inversion Hgt; lia.
-      ++ constructor.
-      + constructor.
-      ++ inversion Hgt; lia.
-      ++ constructor; auto.
-    - apply Forall_cons_iff in Hlt.
-      destruct Hlt.
-      inversion Hl1; clear Hl1; subst.
-      + constructor; try lia.
-      rewrite app_nil_l in IHt. apply IHt; auto; constructor.
-Admitted.
-        
+      + inversion Hlt; clear Hlt; subst; constructor. try lia.
+      -- inversion H. lia.
+      -- constructor.
+      -- inversion H. lia.
+      -- inversion H; clear H; subst; constructor; try lia; auto.
+    - simpl. 
+    inversion Hl2; subst.
+    constructor.
+    + destruct l2 as [|hd tl];  inversion Hlt; subst; try lia.
+    all: inversion Hgt;lia.
+    +  simpl in IHt.
+       apply IHt; auto; constructor.
+    + intros.
+      simpl.
+      assert(Ht: sorted (((y, vy) :: l) ++ (x, Hl1):: l2)); auto.
+    -- apply IHt.
+    +++ inversion Hl2. clear Hl2. subst; auto.
+    +++ apply Forall_cons_iff; split; auto.
+    * inversion Hgt; clear Hgt; subst; auto.
+      inversion H5; clear H5; subst; auto.
+    * inversion Hgt; clear Hgt; subst; auto.
+      inversion H5; clear H5; subst; auto.
+    +++ auto.
+    -- constructor; auto.
+Qed.
 
-    
 
 End Sorted.
